Dafny/Request.dfy
@@ -5,6 +5,8 @@ datatype request = bloodRequest(bloodType: string, volume: int)
 method Request(batchRequest:array<request>, bloodInventory: BloodInventory)
 requires batchRequest != null
 requires bloodInventory != null
+requires bloodInventory.GetArrayVerification() != null
+requires forall i :: 0 <= i < bloodInventory.GetArrayVerification().Length ==> (bloodInventory.GetArrayVerification()[i] != null)
 requires forall i :: 0 <= i < batchRequest.Length ==> (validBloodType(batchRequest[i].bloodType))
 requires forall i :: 0 <= i < batchRequest.Length ==> (batchRequest[i].volume >= bloodInventory.GetBloodCountForBloodTypeVerification(batchRequest[i].bloodType, bloodInventory.GetSizeVerificaiton()))
 {
